\documentclass[a4paper,11pt]{article}

\usepackage{comment}
\usepackage{bbm}
\usepackage{float}
\usepackage{pgfpages}
\usepackage{csquotes}
\usepackage{booktabs}
\usepackage{amsmath,amssymb}
\usepackage{amsthm}
\usepackage{graphicx}
\usepackage{multicol}
\usepackage{mathtools}
\usepackage{mathrsfs}
\usepackage{color}
\usepackage{eucal}
\usepackage{graphicx}
\usepackage{csquotes}
\usepackage{bm}
\usepackage[colorlinks=true, linkcolor=black, urlcolor=black, citecolor=blue]{hyperref}

\newcommand{\argmax}{\mathop{\mathrm{argmax}}\limits}

\title{\vspace{-20mm}Problem Set 1}
\author{29256505 Masato Eguchi}
\date{}

\begin{document}
\maketitle

\section*{2}
$$
\begin{aligned}
(y-g(x))^2 & =E\left[\left[(y-E[y \mid x])+(E[y \mid x]-y(x))]^2 \mid x\right]\right. \\
& =E\left[(y-E[y \mid x])^2+(E[y \mid x]-g(x))^2 \mid x\right] \\
& =E[2(y-E[y \mid x])(E[y \mid x]-g(x)) \mid x] \\
E\left[(y-g(x))^2 \mid x\right] & \left.=E[\{(y-E[y \mid x])+(E[y \mid x]-g(x))\}^2 \mid x\right] \\
& =E\left[(y-E[y \mid x])^2+(E[y \mid x]-g(x))^2 \mid x\right] \\
& +E[2(y-E[y \mid x])(E[y \mid x]-g(x)) \mid x] \\
& \left.=E\left[(y-E[y \mid x])^2+(E[y \mid x]-g(x)\right)^2 \mid x\right] \\
& +E[y E[y \mid x] \mid x]-E[y g(x) \mid x]-E\left[E[y \mid x]^2 \mid x\right]+E[g(x) E[y \mid x] \mid x]
\end{aligned}
$$

Since $E[y \mid x]$ and $g(x)$ are function of $x$,

$$
\begin{aligned}
& E[y E[y \mid x] \mid x]=E[y \mid x] \cdot E[y \mid x] \\
& E[E[y \mid x]^2 \mid x]=E[y \mid x]^2 \\
& E[y g(x) \mid x]=g(x) E[y \mid x] \\
& E[g(x) E[y \mid x] \mid x]=g(x) E[y \mid x]
\end{aligned}
$$

Thus
$$
\begin{aligned}
& E[y E[y \mid x] \mid x]-E[y g(x) \mid x]-E\left[E[y \mid x]^2 \mid x\right]+E[g(x) E[y \mid x] \mid x] \\
& =E[y \mid x]^2-E[y \mid x]^2+g(x) E[y \mid x]-g(x) E[y \mid x] \\
& =0
\end{aligned}
$$

Therefore
$$
\begin{aligned}
& E\left[(y-y(x))^2 \mid x\right]-E\left[(y-E[y \mid x])^2 \mid x\right] \\
& \quad=E\left[(E[y \mid x]-g(x))^2 \mid x\right]=(E[y \mid x]-g(x))^2 \geq 0
\end{aligned}
$$

\section*{4}
We have
\begin{align*}
    (\bm{b}_1',\bm{b}_2')'&=(\bm{X}'\bm{X})^{-1}\bm{X}'\bm{y}\\
    &=\left(\begin{pmatrix}\bm{X}_1'\\\bm{X}_2'\end{pmatrix}(\bm{X}_1,\bm{X}_2)\right)^{-1}\begin{pmatrix}\bm{X}_1'\\\bm{X}_2'\end{pmatrix}\bm{y}\\
    &=\begin{pmatrix}\bm{X}_1'\bm{X}_1&\bm{X}_1'\bm{X}_2\\\bm{X}_2'\bm{X}_1&\bm{X}_2'\bm{X}_2\end{pmatrix}^{-1}\begin{pmatrix}\bm{X}_1'\bm{y}\\\bm{X}_2'\bm{y}\end{pmatrix}\\
    &=\begin{pmatrix}\bm{X}_1'\bm{X}_1&\bm{0}\\\bm{0}&\bm{X}_2'\bm{X}_2\end{pmatrix}^{-1}\begin{pmatrix}\bm{X}_1'\bm{y}\\\bm{X}_2'\bm{y}\end{pmatrix},
\end{align*}
where the last equality follows from the assumption that $\bm{X}_1'\bm{X}_2=\bm{0}$ and $\bm{X}_2'\bm{X}_1=\bm{0}$. Since 
\begin{equation*}
    \begin{pmatrix}\bm{X}_1'\bm{X}_1&\bm{0}\\\bm{0}&\bm{X}_2'\bm{X}_2\end{pmatrix}\begin{pmatrix}(\bm{X}_1'\bm{X}_1)^{-1}&\bm{0}\\\bm{0}&(\bm{X}_2'\bm{X}_2)^{-1}\end{pmatrix}=\bm{I}_k,
\end{equation*}
where $\bm{I}_k$ is a $k\times k$ identity matrix, we have
\begin{align*}
    \begin{pmatrix}\bm{b}_1\\\bm{b}_2\end{pmatrix}&=\begin{pmatrix}(\bm{X}_1'\bm{X}_1)^{-1}&\bm{0}\\\bm{0}&(\bm{X}_2'\bm{X}_2)^{-1}\end{pmatrix}\begin{pmatrix}\bm{X}_1'\bm{y}\\\bm{X}_2'\bm{y}\end{pmatrix}\\
    &=\begin{pmatrix}(\bm{X}_1'\bm{X}_1)^{-1}\bm{X}_1'\bm{y}\\(\bm{X}_2'\bm{X}_2)^{-1}\bm{X}_2'\bm{y}\end{pmatrix}\\
    &=\begin{pmatrix}\widetilde{\bm{b}_1}\\\bm{b}_2\end{pmatrix}.
\end{align*}\qed

\section*{6}
Let $e_i=y_i-\hat{y}_i$. We first show $\sum_{i=1}^n\bm{x}_ie_i=0$. Since we have 
\begin{align*}
    \bm{b}&=(\bm{X}'\bm{X})^{-1}\bm{X}'\bm{Y}\\
    &=\left((\bm{x}_1,\dots,\bm{x}_n)\begin{pmatrix}\bm{x}_1'\\\vdots\\\bm{x}_n'\end{pmatrix}\right)^{-1}(\bm{x}_1,\dots,\bm{x}_n)\begin{pmatrix}y_1\\\vdots\\y_n\end{pmatrix}\\
    &=\left(\sum_{i=1}^n\bm{x}_i\bm{x}_i'\right)^{-1}\left(\sum_{i=1}^n\bm{x}_i y_i\right),
\end{align*}
It follows that 
\begin{align*}
    \sum_{i=1}^n\bm{x}_ie_i&=\sum_{i=1}^n\bm{x}_i(y_i-\hat{y}_i)\\
    &=\sum_{i=1}^n\bm{x}_i\left(y_i-\bm{x}_i'\bm{b}\right)\\
    &=\sum_{i=1}^n\bm{x}_i y_i-\sum_{i=1}^n\bm{x}_i\bm{x}_i'\bm{b}\\
    &=\sum_{i=1}^n\bm{x}_i y_i-\sum_{i=1}^n\bm{x}_i\bm{x}_i'\left(\sum_{j=1}^n\bm{x}_j\bm{x}_j'\right)^{-1}\left(\sum_{j=1}^n\bm{x}_j y_j\right)\\
    &=\sum_{i=1}^n\bm{x}_i y_i-\sum_{i=1}^n\bm{x}_i y_i\\
    &=\bm{0}.
\end{align*}
Thus, we have 
\begin{align*}
    \sum_{i=1}^n\hat{y}_ie_i&=\sum_{i=1}^n\bm{x}_i'\bm{b}e_i\\
    &=\sum_{i=1}^n\bm{b}'\bm{x}_ie_i\\
    &=\bm{b}'\sum_{i=1}^n\bm{x}_ie_i\\
    &=0.
\end{align*}
Also, let $\bar{\hat{y}}=\frac{1}{n}\sum_{i=1}^n\hat{y}_i$. Then we have
\begin{align*}
    \bar{\hat{y}}&=\frac{1}{n}\sum_{i=1}^n\hat{y}_i\\
    &=\frac{1}{n}\sum_{i=1}^n(y_i-e_i)\\
    &=\frac{1}{n}\sum_{i=1}^ny_i-\frac{1}{n}\sum_{i=1}^ne_i\\
    &=\bar{y}.
\end{align*}
Now, denote the sample correlation coefficient between $y_i$ and $\hat{y}_i$ by $r$. We have
\begin{align*}
    r^2&=\left(\frac{\sum_{i=1}^n(y_i-\bar{y})(\hat{y}_i-\bar{\hat{y}})}{\sqrt{\sum_{i=1}^n(y_i-\bar{y})^2\sum_{i=1}^n(\hat{y}_i-\bar{\hat{y}})^2}}\right)^2\\
    &=\left(\frac{\sum_{i=1}^n(y_i-\bar{y})(\hat{y}_i-\bar{y})}{\sqrt{\sum_{i=1}^n(y_i-\bar{y})^2\sum_{i=1}^n(\hat{y}_i-\bar{y})^2}}\right)^2\\
    &=\left(\frac{\sum_{i=1}^n(\hat{y}_i+e_i-\bar{y})(\hat{y}_i-\bar{y})}{\sqrt{\sum_{i=1}^n(y_i-\bar{y})^2\sum_{i=1}^n(\hat{y}_i-\bar{y})^2}}\right)^2\\
    &=\left(\frac{\sum_{i=1}^n(\hat{y}_i-\bar{y})^2+\sum_{i=1}^ne_i(\hat{y}_i-\bar{y})}{\sqrt{\sum_{i=1}^n(y_i-\bar{y})^2\sum_{i=1}^n(\hat{y}_i-\bar{y})^2}}\right)^2\\
    &=\left(\frac{\sum_{i=1}^n(\hat{y}_i-\bar{y})^2+\sum_{i=1}^n\hat{y}_ie_i-\bar{y}\sum_{i=1}^ne_i}{\sqrt{\sum_{i=1}^n(y_i-\bar{y})^2\sum_{i=1}^n(\hat{y}_i-\bar{y})^2}}\right)^2\\
    &=\frac{\left(\sum_{i=1}^n(\hat{y}_i-\bar{y})^2\right)^2}{\sum_{i=1}^n(y_i-\bar{y})^2\sum_{i=1}^n(\hat{y}_i-\bar{y})^2}\\
    &=\frac{\sum_{i=1}^n(\hat{y}_i-\bar{y})^2}{\sum_{i=1}^n(y_i-\bar{y})^2}\\
    &=R^2.
\end{align*}

\section*{8}
Let $S\left(\tilde{\beta_1}, \tilde{\beta_2}\right)=\sum_{i=1}^n\left(y_i-\tilde{\beta_1}-\tilde{\beta_2} x_i\right)^2$
$$
\left(\hat{\beta}_1, \hat{\beta}_2\right)=\underset{\tilde{\beta}_1, \hat{\beta}_2}{\operatorname{argmin}} S
$$
First-order condition is
$$
\begin{aligned}
\frac{\partial S}{\partial \tilde{\beta}_1} & =2 \sum_{i=1}^n\left(\tilde{\beta_1}-y_i+\tilde{\beta_2} x_i\right) \\
& =2\left(\tilde{\beta_1}-\frac{1}{n} \sum_{i=1}^n y_i+\frac{1}{n} \sum_{i=1}^n \tilde{\beta_2} x_i\right)=0 \\
\frac{\partial S}{\partial \tilde{\beta}_2} & =2 \sum_{i=1}^n\left(x_i \tilde{\beta}_1-y_i x_i+\tilde{\beta}_2 x_i^2\right)
\end{aligned}
$$
Substitute $n \tilde{\beta_1}=\sum_{i=1}^n y_i-\sum_{i=1}^n \tilde{\beta}_2 x_i$ into $\frac{\partial S}{\partial \tilde{\beta}_2}$
$$
\begin{aligned}
& \sum_{i=1}^n x_i y_i-x_i^2 \tilde{\beta}_2-x_i\left(\sum_{i=1}^n y_i^n-\sum_{i=1}^n \tilde{\beta}_2 x_i\right)=0 \\
& \begin{aligned}
\tilde{\beta}_2 & =\frac{n \sum_{i=1}^n x_1 y_i-\sum_{i=1}^n x_i \sum_{i=1}^n y_i}{n \sum_{i=1}^n x_i^2-\left(\sum_{i=1}^n x_i\right)^2} \\
n \sum_{i=1}^n x_i y_i-\sum_{i=1}^n x_i \sum_{i=1}^n y_i & =n \sum_{i=1}^n x_i y_i-\sum_{i=1}^n x_i \sum_{i=1}^n y_i+\sum_{i=1}^n x_i \sum_{i=1}^n y_i-\sum_{i=1}^n x_i \sum_{i=1}^n y_i \\
& =n \sum_{i=1}^n x_i y_i-n \bar{x} \sum_{i=1}^n y_i - n \bar{y} \sum_{i=1}^n x_i+n^2 \bar{x} \bar{y} \\
& =n \sum_{i=1}^n\left(x_i-\bar{x}\right)\left(y_i-\bar{y}\right)
\end{aligned} \\
& \begin{aligned}
n \sum_{i=1}^n x_i^2-\left(\sum_{i=1}^n x_i\right)^2 & =n \sum_{i=1}
^n x_i^2-2\left(\sum_{i=1}^n x_i\right)^2+\left(\sum_{i=1}^n x_i\right)^2 \\
& =n \sum_{i=1}^n x_i^2-2 n \bar{x} \sum_{i=1}^n x_i=n^2 \bar{x}^2 \\
& =n \sum_{i=1}^n\left(x_i-\bar{x}\right)^2 \\
\end{aligned} \\
& \tilde{\beta}_2=\frac{\sum_{i=1}^n\left(x_i-\bar{x}\right)\left(y_i-\bar{y}\right)}{\sum_{i=1}^n\left(x_i-\bar{x}\right)^2}
\end{aligned}
$$
Since $\frac{\partial S}{\partial \tilde{\beta}_1}$ and $\frac{\partial S}{\partial \tilde{\beta}_2}$ monotonically increasing, $S$ has a minimum value at $\tilde{\beta}_2=\frac{\sum_{i=1}^n\left(x_i-\bar{x}\right)\left(y_i-\bar{y}\right)}{\sum_{i=1}^n\left(x_i-\bar{x}\right)^2}$
Therefore 
$$
\hat{\beta}_2=\frac{\sum_{i=1}^n\left(x_i-\bar{x}\right)\left(y_i-\bar{y}\right)}{\sum_{i=1}^n\left(x_i-\bar{x}\right)^2}
$$

\end{document}